refactoring

theories/FMset/FMsetTC.v
@@ -7,7 +7,7 @@
 
 (* 
   Problem:
-    Finite multiset constraint solvability (FMsetC)
+    Finite multiset term constraint solvability (FMsetTC)
 
   Finite multisets with one constant 0 and one unary constructor h
   A finite multiset A is represented by a list of its elements.
@@ -25,7 +25,7 @@
     φ(t ⊍ u) = φ(t) ++ φ(u)
     φ(h (t)) = map h (φ(t))
 
-  FMsetC:
+  FMsetTC:
     Given a list (t₁ ≐ u₁),...,(tₙ ≐ uₙ) of constraints,
     is there a valuation φ : nat -> list nat such that
     φ(t₁) ≡ φ(u₁),..., φ(tₙ) ≡ φ(uₙ),
@@ -40,10 +40,7 @@ Require Import PeanoNat.
 Require Import List.
 Import ListNotations.
 
-(* list equality up to permutation *)
-Definition mset_eq (A B: list nat) : Prop := 
-  forall c, count_occ Nat.eq_dec A c = count_occ Nat.eq_dec B c.
-Notation "A ≡ B" := (mset_eq A B) (at level 65).
+From Undecidability Require Import Problems.FMsetC.
 
 (* terms *)
 Inductive mset_term : Set :=
@@ -62,29 +59,8 @@ Fixpoint mset_sem (φ : nat -> list nat) (A : mset_term) : list nat :=
   end.
 
 (* list of constraints *)
-Definition FMsetC_PROBLEM := list (mset_term * mset_term).
+Definition FMsetTC_PROBLEM := list (mset_term * mset_term).
 
 (* is there a valuation φ that satisfies all contraints *)
-Definition FMsetC_SAT (l : FMsetC_PROBLEM) := 
+Definition FMsetTC_SAT (l : FMsetTC_PROBLEM) := 
   exists (φ : nat -> list nat), forall (A B : mset_term), In (A, B) l -> (mset_sem φ A) ≡ (mset_sem φ B).
-
-
-(* elementary mset constraints *)
-Inductive msetc : Set :=
-  | msetc_zero : nat -> msetc
-  | msetc_sum : nat -> nat -> nat -> msetc
-  | msetc_h : nat -> nat -> msetc.
-
-Definition msetc_sem (φ: nat -> list nat) (c: msetc) :=
-  match c with
-    | msetc_zero x => φ x ≡ [0]
-    | msetc_sum x y z => φ x ≡ (φ y) ++ (φ z)
-    | msetc_h x y => φ x ≡ map S (φ y)
-  end.
-
-(* list of elementary constraints *)
-Definition FMsetEC_PROBLEM := list msetc.
-
-(* given a list l of elementary constraints, 
-  is there a valuation φ satisfying each elementary constraint? *)
-Definition FMsetEC_SAT (l : FMsetEC_PROBLEM) := exists φ, forall c, In c l -> msetc_sem φ c.
