theories/Problems/FMsetC.v
@@ -9,26 +9,26 @@
   Problem:
     Finite multiset constraint solvability (FMsetC)
 
-  Finite multisets with one constant 0 and one unary constructor h
+  Finite multisets with one constant 0 and one unary constructor h.
   A finite multiset A is represented by a list of its elements.
   The element (h^n 0) is represented by the natural number n.
 
-  Terms t, u:
-    t, u ::= zero | t ⊍ u | h (t) | x : nat
-    where x ranges over multiset variables
-  
-  Constraints:
-    t ≐ u 
+  Constraints are of shape:
+    x ≐ [0]
+    x ≐ y ⊍ z
+    x ≐ h (y) 
 
-  Term Interpretation:
-    φ(zero) = [0]
-    φ(t ⊍ u) = φ(t) ++ φ(u)
-    φ(h (t)) = map h (φ(t))
+  Constraint semantics:
+    φ(y ⊍ z) = φ(y) ++ φ(z)
+    φ(h (y)) = map h (φ(y))
 
   FMsetC:
-    Given a list (t₁ ≐ u₁),...,(tₙ ≐ uₙ) of constraints,
+    Given a list of constraints,
     is there a valuation φ : nat -> list nat such that
-    φ(t₁) ≡ φ(u₁),..., φ(tₙ) ≡ φ(uₙ),
+    for each constraint c we have
+      if c is x ≐ [0], then φ(x) ≡ [0]
+      if c is x ≐ y ⊍ z, then φ(x) ≡ φ(y) ++ φ(z)
+      if c is x ≐ h (y), then φ(x) ≡ map S (φ(y))
     where ≡ is equality up to permutation?
   
   References:
@@ -45,36 +45,13 @@ Definition mset_eq (A B: list nat) : Prop :=
   forall c, count_occ Nat.eq_dec A c = count_occ Nat.eq_dec B c.
 Notation "A ≡ B" := (mset_eq A B) (at level 65).
 
-(* terms *)
-Inductive mset_term : Set :=
-  | mset_term_zero : mset_term
-  | mset_term_var : nat -> mset_term
-  | mset_term_plus : mset_term -> mset_term -> mset_term
-  | mset_term_h : mset_term -> mset_term.
-
-(* evaluate an mset wrt. a valuation φ *)
-Fixpoint mset_sem (φ : nat -> list nat) (A : mset_term) : list nat :=
-  match A with
-    | mset_term_zero => [0]
-    | mset_term_var x => φ x
-    | mset_term_plus A B => (mset_sem φ A) ++ (mset_sem φ B)
-    | mset_term_h A => map S (mset_sem φ A)
-  end.
-
-(* list of constraints *)
-Definition FMsetC_PROBLEM := list (mset_term * mset_term).
-
-(* is there a valuation φ that satisfies all contraints *)
-Definition FMsetC_SAT (l : FMsetC_PROBLEM) := 
-  exists (φ : nat -> list nat), forall (A B : mset_term), In (A, B) l -> (mset_sem φ A) ≡ (mset_sem φ B).
-
-
-(* elementary mset constraints *)
+(* mset constraints *)
 Inductive msetc : Set :=
   | msetc_zero : nat -> msetc
   | msetc_sum : nat -> nat -> nat -> msetc
   | msetc_h : nat -> nat -> msetc.
 
+(* mset constraint semantic *)
 Definition msetc_sem (φ: nat -> list nat) (c: msetc) :=
   match c with
     | msetc_zero x => φ x ≡ [0]
@@ -83,8 +60,8 @@ Definition msetc_sem (φ: nat -> list nat) (c: msetc) :=
   end.
 
 (* list of elementary constraints *)
-Definition FMsetEC_PROBLEM := list msetc.
+Definition FMsetC_PROBLEM := list msetc.
 
 (* given a list l of elementary constraints, 
   is there a valuation φ satisfying each elementary constraint? *)
-Definition FMsetEC_SAT (l : FMsetEC_PROBLEM) := exists φ, forall c, In c l -> msetc_sem φ c.
+Definition FMsetC_SAT (l : FMsetC_PROBLEM) := exists φ, forall c, In c l -> msetc_sem φ c.
